BoogieOutputs/request.bpl
@@ -62,15 +62,15 @@ implementation pop()
     $sp := ($sp) - (1);
 }
 
-var Counter: real;
-const Max: real;
+const MAX_REQUESTS: real;
 
-axiom((Max) == (100.0));
+axiom((MAX_REQUESTS) == (10.0));
+var active_requests: real;
 procedure initGlobals();
-modifies Counter;
+modifies active_requests;
 implementation initGlobals()
 {
-    Counter := 41.0;
+    active_requests := 0.0;
 }
 
 procedure {:inline true} popArgs1() returns (a1: real);
@@ -83,15 +83,17 @@ implementation popArgs1() returns (a1: real)
     a1 := $stack[$sp];
 }
 
-procedure inc_and_check();
+procedure acquire_request();
 modifies $tmp1;
 modifies $tmp2;
 modifies $tmp3;
 modifies $sp;
 modifies $stack;
-modifies Counter;
-implementation inc_and_check()
+modifies active_requests;
+implementation acquire_request()
 {
+    var loc1: real;
+    var loc2: real;
     var idx: int;
     var entry_sp: int;
     var load_i: int;
@@ -100,16 +102,67 @@ implementation inc_and_check()
     $tmp1 := 0.0;
     $tmp2 := 0.0;
     $tmp3 := 0.0;
-    call push(Counter);
-    call push(1.0);
+    loc1 := 0.0;
+    loc2 := 0.0;
+    call push(active_requests);
+    call loc1 := popArgs1();
+    call push(loc1);
+    call push(MAX_REQUESTS);
     call popToTmp1();
     call popToTmp2();
-    call push(($tmp2) + ($tmp1));
-    call Counter := popArgs1();
-    call push(Counter);
-    call push(Max);
+    call push(bool_to_real(($tmp2) >= ($tmp1)));
+    call popToTmp1();
+    if (real_to_bool($tmp1)) {
+        call push(0.0);
+        call loc2 := popArgs1();
+    } else {
+        call push(loc1);
+        call push(1.0);
+        call popToTmp1();
+        call popToTmp2();
+        call push(($tmp2) + ($tmp1));
+        call active_requests := popArgs1();
+        call push(1.0);
+        call loc2 := popArgs1();
+block_end_1:
+    }
+    call push(loc2);
+}
+
+procedure release_request();
+modifies $tmp1;
+modifies $tmp2;
+modifies $tmp3;
+modifies $sp;
+modifies $stack;
+modifies active_requests;
+implementation release_request()
+{
+    var loc1: real;
+    var idx: int;
+    var entry_sp: int;
+    var load_i: int;
+    var store_i: int;
+    entry_sp := $sp;
+    $tmp1 := 0.0;
+    $tmp2 := 0.0;
+    $tmp3 := 0.0;
+    loc1 := 0.0;
+    call push(active_requests);
+    call loc1 := popArgs1();
+    call push(loc1);
+    call push(0.0);
     call popToTmp1();
     call popToTmp2();
-    call push(bool_to_real(($tmp2) < ($tmp1)));
+    call push(bool_to_real(($tmp2) > ($tmp1)));
+    call popToTmp1();
+    if (real_to_bool($tmp1)) {
+        call push(loc1);
+        call push(1.0);
+        call popToTmp1();
+        call popToTmp2();
+        call push(($tmp2) - ($tmp1));
+        call active_requests := popArgs1();
+    }
 }
 
